src/extensions/paths/OperationalSemantics.v
@@ -5,34 +5,34 @@ Require Import Definitions Binding Lookup.
 
 (** * Operational Semantics *)
 
-Reserved Notation "t1 '⤳' t2" (at level 40, t2 at level 39).
+Reserved Notation "t1 '⟼' t2" (at level 40, t2 at level 39).
 
 Inductive red : sta * trm -> sta * trm -> Prop :=
 
 (** [s ∋ (p, lambda(T)t)  ]      #<br>#
     [―――――――――――――――――――――]      #<br>#
-    [(s, p q) ⤳ (s, t^q)]      *)
+    [(s, p q) ⟼ (s, t^q)]      *)
 | red_app: forall s p q T t,
     s ∋ (p, λ(T) t) ->
-    (s, trm_app p q) ⤳ (s, open_trm_p q t)
+    (s, trm_app p q) ⟼ (s, open_trm_p q t)
 
-(** [(s, let x = v in t) ⤳ ((s, x = v), t^x)] *)
+(** [(s, let x = v in t) ⟼ ((s, x = v), t^x)] *)
 | red_let_val : forall v t s x,
     x # s ->
-    (s, trm_let (trm_val v) t) ⤳ (s & x ~ v, open_trm x t)
+    (s, trm_let (trm_val v) t) ⟼ (s & x ~ v, open_trm x t)
 
-(** [(s, let y = p in t) ⤳ (s, t^p)] *)
+(** [(s, let y = p in t) ⟼ (s, t^p)] *)
 | red_let_path : forall t s p,
-    (s, trm_let (trm_path p) t) ⤳ (s, open_trm_p p t)
+    (s, trm_let (trm_path p) t) ⟼ (s, open_trm_p p t)
 
-(** [(s, t0) ⤳ (s', t0')]                            #<br>#
+(** [(s, t0) ⟼ (s', t0')]                            #<br>#
     [―――――――――――――――――――――――――――――――――――――――――――――――]  #<br>#
-    [(s, let x = t0 in t) ⤳ (s', let x = t0' in t)]  *)
+    [(s, let x = t0 in t) ⟼ (s', let x = t0' in t)]  *)
 | red_let_tgt : forall t0 t s t0' s',
-    (s, t0) ⤳ (s', t0') ->
-    (s, trm_let t0 t) ⤳ (s', trm_let t0' t)
+    (s, t0) ⟼ (s', t0') ->
+    (s, trm_let t0 t) ⟼ (s', trm_let t0' t)
 
-where "t1 '⤳' t2" := (red t1 t2).
+where "t1 '⟼' t2" := (red t1 t2).
 
 (** ** Normal forms *)
 
